\documentclass[10pt,a4paper,landscape]{article}
\input{preamble}

\begin{document}
% Suppress page number for all pages
\pagestyle{empty}

% Each section goes into this env
\begin{multicols*}{3}
\section*{Eliminate left-recursion by converting it to right recursion}
\begin{itemize}
\item Suppose the following grammar ($\beta$ \emph{does not} start with $A$):
  \[
A\to A\alpha \gor \beta
  \]
\item Recursively applying $A$, we can have the following string
  \[
s = A\alpha \to A\alpha\alpha \overset{*}{\to} \beta\underbracket[0.5pt][3pt]{\alpha\cdots\alpha}_{\alpha^{*}} = \beta\alpha^{*}
  \]
\item Then grammar $A$ is equivalent to $A' \to\beta\alpha^{*}$ and thus
  \begin{align*}
    A\to &\; \beta A' \\
    A'\to &\; \alpha A'\gor \varepsilon
  \end{align*}
\end{itemize}
\section*{A simple example}
\begin{align*}
  E\to &\; E + T \\
  E\to &\; T
\end{align*}
\begin{enumerate}
\item since $E\to E + T\gor T$, we have $\beta = T$
\item since $E \overset{*}{\to} T (+ T)^{*}$, we have $E' = (+ T)^{*} = + T E' \gor \varepsilon$
\begin{align*}
  E\to &\; T E' \\
  E'\to &\; + T E' \gor \varepsilon
\end{align*}
\end{enumerate}
\section*{Multiple left recursions}
\begin{align*}
  A\to &\; A\alpha_1\gor A\alpha_2 \gor \cdots \gor A\alpha_n & (n \geq 0)\\
  A\to &\; \beta_1\gor\beta_2\gor\cdots\gor\beta_m  & (m \geq 0)
\end{align*}
The above grammar can be re-written as follows:
\begin{align*}
  A\to &\; \beta_1 A'\gor\beta_2 A'\gor\cdots\gor\beta_m A'  & (m \geq 0) \\
  A'\to &\; \alpha_1 A'\gor \alpha_2 A' \gor \cdots \gor \alpha_n A' & (n \geq 0) \\
  A'\to &\; \varepsilon
\end{align*}
\section*{A simple example}
\[
\begin{pmatrix}
  X\to&\; X \gamma_1 \\
  X\to&\; X \gamma_2 \\
  \cdots             \\
  X\to&\; X \gamma_n \\
  X\to&\; \alpha_1   \\
  X\to&\; \alpha_2   \\
  \cdots             \\
  X\to&\; \alpha_m
\end{pmatrix}
\implies
\begin{pmatrix}
  X\to&\; \alpha_1 X' \\
  X\to&\; \alpha_2 X' \\
  \cdots             \\
  X\to&\; \alpha_m X' \\
  X'\to&\;\gamma_1 X' \\
  X'\to&\; \gamma_2 X' \\
  \cdots             \\
  X'\to&\; \gamma_n X' \\
  X'\to&\; \varepsilon
\end{pmatrix}
\]
\section*{Remove indirect left-recursions: an example}
\begin{minipage}{.5\linewidth}
\begin{align}
  S\to &\; Q \\
  Q\to &\; QED \gor q \\
  D\to &\; NFA \gor d \\
  N\to &\; DFA \gor n
\end{align}
\end{minipage}
\begin{minipage}{.5\linewidth}
\begin{align}
  A\to & a \\
  E\to &\; e \gor \varepsilon \\
  F\to &\; f
\end{align}
\end{minipage}
\section*{Step 1: Re-arrange grammar in terms of dependencies}
\begin{align*}
  Q\to &\; QED \gor q & (1)\\
  E\to &\; e \gor \varepsilon &(2) \\
  D\to &\; NFA \gor d & (\mr{3})\\
  N\to &\; DFA \gor n & (\mr{4})\\
  F\to &\; f          & (5)\\
  A\to &\; a            & (6)
\end{align*}
\section*{Step 2: Turn indirect left-recursion into direct one}
$(\mr{3})$ and $(\mr{4})$ show $ D\to N\to D$ (indirect) and thus:
\begin{align*}
  Q\to &\; QED \gor q & (1)\\
  E\to &\; e \gor \varepsilon &(2) \\
  D\to &\; \mb{DFA}\mo{FA} \gor \mb{n}\mo{FA} \gor d &(\mr{3})\\
  F\to &\; f          & (5)\\
  A\to &\; a          & (6)
\end{align*}

\end{multicols*}
\end{document}
