% Q1N1
If assume the list \texttt{xs} is empty \texttt{[]}, then \((\dagger)\) becomes:
\begin{lstlisting}
length([] ++ []) = length (dupAll([])) -- Assumption
                 = length []           -- D2
\end{lstlisting}
So it seems if I can have
\begin{lstlisting}
length([] ++ []) = length [] + length []
\end{lstlisting}
or more generally
\begin{lstlisting}
length(xs ++ ys) = length xs + length ys
\end{lstlisting}
I can use this lemma to complete the proof of \((\dagger)\).  Therefore, the needed lemma is
\[
  \forall\verb|xs|.\,\forall\verb|ys|.\:\:
 \verb|length (xs ++ ys) = length xs + length ys|
\]
