% Q1N2
I need to show that
\[
  \forall\verb|xs|.\,\forall\verb|ys|.\:\:
 \verb|length (xs ++ ys) = length xs + length ys|
\]
Let \texttt{ys} be an arbitrary list and treat \texttt{ys} as a constant and then I need to show that
\[
  \forall\verb|xs|.\:\:
 \verb|length (xs ++ ys) = length xs + length ys|
\]
\textbf{Base Case.} I need to show that
\[
 \verb|length ([] ++ ys) = length [] + length ys|
\]
\begin{lstlisting}
  length ([] ++ ys) = length ys                -- A1
                    = 0 + length ys            -- Arithmetic
                    = length [] + length ys    -- L1
\end{lstlisting}
\textbf{Step Case.} I need to show that
\[
  \forall\verb|xs|.\,\forall\verb|ys|.\:\:
 \verb|length (xs ++ ys) = length xs + length ys|
\]
Let \texttt{x} be an arbitrary list element and \texttt{xs}, an arbitrary non-empty list, and assume the inductive hypothesis as
\begin{equation*}
  \verb|length (xs + ys) = length xs ++ length ys| \tag{IH}
\end{equation*}
Then I need to show that
\begin{equation*}
  \verb|length ((x:xs) + ys) = length (x:xs) ++ length ys|
\end{equation*}
It is easier to prove this by starting with RHS:
\begin{lstlisting}
  length (x:xs) + length ys = 1 + length xs + length ys   -- L1
                            = 1 + length (xs ++ ys)       -- IH
                            = length (x:(xs ++ ys))       -- L2
                            = length ((x:xs) ++ ys)       -- A2
\end{lstlisting}
thus this finishes the proof and I now get
\begin{equation*}
  \forall\verb|xs|.\,\forall\verb|ys|.\:\:
  \verb|length (xs ++ ys) = length xs + length ys| \tag{\texttt{Lemma}}
\end{equation*}
