% Q1N3
I need to show that
\begin{equation*}
  \forall\verb|xs|.\:\:
  \verb|length (xs ++ xs) = length (dupAll xs)|
\end{equation*}
\textbf{Base Case.} When \texttt{xs} is an empty list \texttt{[]}, I need to show
\begin{equation*}
  \verb|length ([] ++ []) = length (dupAll [])|
\end{equation*}
This is easy to prove
\begin{lstlisting}
  length ([] ++ [])  = length [] + length []  -- Lemma
                     = 0 + 0                  -- L1
                     = 0                      -- Arithmetic
                     = length []              -- L1
                     = length (dupAll [])     -- D1
\end{lstlisting}
\textbf{Step Case.} Now let \texttt{x} be an arbitrary list element and \texttt{xs} an arbitrary list, and assume that
\begin{equation*}
  \verb|length (xs ++ xs) = length (dupAll xs)| \tag{IH}
\end{equation*}
I need to show that
\begin{equation*}
  \verb|length ((x:xs) ++ (x:xs)) = length (dupAll (x:xs))|
\end{equation*}
\begin{lstlisting}
  length (dupAll (x:xs)) = length (x:x:(dupAll xs))       -- D2
                         = 1 + length (x:(dupAll xs))     -- L2
                         = 1 + 1 + length (xs ++ xs)      -- IH
                         = 1 + 1 + length xs + length xs  -- Lemma
                         = 1 + length xs + 1 + length xs  -- Commutativity
                         = length (x:xs) + length (x:xs)  -- L2
                         = length ((x:xs) + (x:xs))       -- Lemma
\end{lstlisting}
which finishes the proof.
