\documentclass[10pt,a4paper,landscape]{article}
\input{preamble}

\begin{document}
% Suppress page number for all pages
\pagestyle{empty}

% Each section goes into this env
\begin{multicols*}{3}
\section*{Eliminate left-recursion by converting it to right recursion}
\begin{itemize}
\item Suppose the following grammar ($\beta$ \emph{does not} start with $A$):
  \[
A\to A\alpha \gor \beta
  \]
\item Recursively applying $A$, we can have the following string
  \[
s = A\alpha \to A\alpha\alpha \overset{*}{\to} \beta\underbracket[0.5pt][3pt]{\alpha\cdots\alpha}_{\alpha^{*}} = \beta\alpha^{*}
  \]
\item Then grammar $A$ is equivalent to $A' \to\beta\alpha^{*}$ and thus
  \begin{align*}
    A\to &\; \beta A' \\
    A'\to &\; \alpha A'\gor \varepsilon
  \end{align*}
\end{itemize}
\section*{A simple example}
\begin{align*}
  E\to &\; E + T \\
  E\to &\; T
\end{align*}
\begin{enumerate}
\item since $E\to E + T\gor T$, we have $\beta = T$
\item since $E \overset{*}{\to} T (+ T)^{*}$, we have $E' = (+ T)^{*} = + T E' \gor \varepsilon$
\begin{align*}
  E\to &\; T E' \\
  E'\to &\; + T E' \gor \varepsilon
\end{align*}
\end{enumerate}
\section*{Multiple left recursions}
\begin{align*}
  A\to &\; A\alpha_1\gor A\alpha_2 \gor \cdots \gor A\alpha_n & (n \geq 0)\\
  A\to &\; \beta_1\gor\beta_2\gor\cdots\gor\beta_m  & (m \geq 0)
\end{align*}
The above grammar can be re-written as follows:
\begin{align*}
  A\to &\; \beta_1 A'\gor\beta_2 A'\gor\cdots\gor\beta_m A'  & (m \geq 0) \\
  A'\to &\; \alpha_1 A'\gor \alpha_2 A' \gor \cdots \gor \alpha_n A' & (n \geq 0) \\
  A'\to &\; \varepsilon
\end{align*}
\section*{A simple example}
\[
\begin{pmatrix}
  X\to&\; X \gamma_1 \\
  X\to&\; X \gamma_2 \\
  \cdots             \\
  X\to&\; X \gamma_n \\
  X\to&\; \alpha_1   \\
  X\to&\; \alpha_2   \\
  \cdots             \\
  X\to&\; \alpha_m
\end{pmatrix}
\implies
\begin{pmatrix}
  X\to&\; \alpha_1 X' \\
  X\to&\; \alpha_2 X' \\
  \cdots             \\
  X\to&\; \alpha_m X' \\
  X'\to&\;\gamma_1 X' \\
  X'\to&\; \gamma_2 X' \\
  \cdots             \\
  X'\to&\; \gamma_n X' \\
  X'\to&\; \varepsilon
\end{pmatrix}
\]
\section*{Remove indirect left-recursions: an example}
\begin{minipage}{.5\linewidth}
\begin{align}
  S\to &\; Q \\
  Q\to &\; QED \gor q \\
  D\to &\; NFA \gor d \\
  N\to &\; DFA \gor n
\end{align}
\end{minipage}
\begin{minipage}{.5\linewidth}
\begin{align}
  A\to & a \\
  E\to &\; e \gor \varepsilon \\
  F\to &\; f
\end{align}
\end{minipage}
\section*{Step 1: Re-arrange grammar in terms of dependencies}
\begin{align*}
  Q\to &\; QED \gor q & (1)\\
  E\to &\; e \gor \varepsilon &(2) \\
  D\to &\; NFA \gor d & (\mb{3})\\
  N\to &\; DFA \gor n & (\mo{4})\\
  F\to &\; f          & (5)\\
  A\to &\; a            & (6)
\end{align*}
\section*{Step 2: Turn indirect left-recursion into direct one}
\begin{itemize}
\item $(\mb{3})$ and $(\mo{4})$ show $ D\to N\to D$ (\mr{indirect} left recursion)
\item turn it into \mr{direct} left recursion $(\mb{3})$ by \mr{substitution}
\end{itemize}
\begin{align*}
  Q\to &\; QED \gor q & (1)\\
  E\to &\; e \gor \varepsilon &(2) \\
  D\to &\; \mo{DFA}\mb{FA} \gor \mo{n}\mb{FA} \gor d &(\mb{3})\\
  F\to &\; f          & (5)\\
  A\to &\; a          & (6)
\end{align*}
\section*{Step 3: Remove direct left-recursion(s)}
\begin{itemize}
\item Production $(1)$ has direct left-recursion with below format:
  \[
    Q\to \; Q\overbracket[0.5pt][2pt]{ED}^{\alpha} \gor \overbracket[0.5pt][3pt]{q}^{\beta}
  \]
\item Eliminate the left-recursion by rewriting it to:
  \begin{align*}
    Q\to &\; q Q' & (1)\\
    Q'\to &\; EDQ' \gor \varepsilon &(2)
  \end{align*}
\item Production $(3)$ has direct left-recursion with below format:
  \[
    D\to \; D\overbracket[0.5pt][2pt]{FAFA}^{\alpha} \gor \overbracket[0.5pt][2pt]{nFA}^{\beta_1} \overbracket[0.5pt][4.5pt]{q}^{\beta_2}
  \]
\item Eliminate left-recursion in $(3)$ and keep other productions:
  \begin{align*}
    D\to &\; nFA D' \gor d D' & (3)\\
    D'\to &\; FAFAD' \gor \varepsilon &(4)\\
    F\to &\; f          & (5)\\
    A\to &\; a          & (6)\\
    E\to &\; e \gor \varepsilon &(7)
  \end{align*}
\end{itemize}
\section*{Left refactoring}
\begin{itemize}
\item A grammar where the RHS share common prefix ($\alpha \neq \varepsilon$)
\[
  A\to \alpha\beta_1 \gor \alpha\beta_2 \gor \cdots \gor \alpha\beta_n
\]
\item backtracking and lookahead $\to$ overhead + slow compilation
\item \mo{solution}: re-write the production to the following
  \begin{align*}
    A\to &\; \alpha A' \\
    A'\to &\; \beta_1 \gor \beta_2 \gor \cdots \gor \beta_n
  \end{align*}
\end{itemize}
\section*{Example 1}
\begin{enumerate}[start=0]
\item Given a grammar with the following productions
  \begin{align*}
    E\to &\; T + E \gor T \\
    T\to &\; \textsf{int} \gor \textsf{int} * T \\
    T\to &\; (E)
  \end{align*}
\item identify \mb{common} prefix(es)
  \begin{align*}
    E\to &\; \mb{T} + E \gor \mb{T} \\
    T\to &\; \mb{\textsf{int}} \gor \mb{\textsf{int}} * T \\
    T\to &\; (E)
  \end{align*}
\item re-write the grammar to remove \mb{common} prefix(es)
  \begin{align*}
    E\to &\; \mb{T} E'\\
    E'\to &\; + E \gor \varepsilon \\
    T\to &\; \mb{\textsf{int}}\,T' \\
    T'\to &\; \mb{\textsf{int}} * T \gor \varepsilon \\
    T\to &\; (E)
  \end{align*}
\end{enumerate}
\section*{Example 2}
\begin{enumerate}
\item Identify the \mb{common} prefix(es)
  \begin{align*}
    \textsf{stmt} \to &\quad \textsf{\mb{if expr then stmt} else stmt} \\
                      &\gor \mb{\textsf{if expr then stmt}}
  \end{align*}
\item re-write the grammar to remove \mb{common} prefix(es)
  \begin{align*}
    \textsf{stmt} \to &\quad \textsf{if expr then stmt}\; E' &(1) \\
     E'\to &\quad \textsf{else stmt} \gor \varepsilon        &(2)
  \end{align*}
\item $(2)$ is still ambiguous but it's easy to tell $\varepsilon$ from non-empty
\end{enumerate}
\end{multicols*}
\end{document}
