\documentclass[10pt,a4paper,landscape]{article}

% -- Layout ----
\usepackage[top=1cm, bottom=1cm, left=0.5cm, right=0.5cm, landscape]{geometry}

% -- Titles ----
\usepackage[
  tiny,                     % text size title
  compact                   % reduce vertical space before/after title
]{titlesec}
% \titlespacing*

% -- Colors ----
\usepackage[dvipsnames]{xcolor}
\definecolor{gr}{HTML}{008000}
\definecolor{bl}{HTML}{2020C0}

% -- Lists -----
\usepackage[inline]{enumitem}
\setlist{noitemsep}

% -- Code listing ---
\usepackage{listings}
\lstset{
  aboveskip=3pt,
  belowskip=3pt,
  basicstyle=\small\ttfamily,
  commentstyle=\upshape\ttfamily,
  frame=single,
  language=Haskell,
}

% -- Multi Columns --
\usepackage{multicol}

% -- Global spacing settings ----
\setlength{\abovedisplayskip}{3pt}
\setlength{\belowdisplayskip}{3pt}
\setlength{\abovedisplayshortskip}{3pt}
\setlength{\belowdisplayshortskip}{3pt}
\setlength{\parindent}{0pt}
\setlength{\parskip}{0pt plus 0.5ex}
\begin{document}
% Suppress page number for all pages
\pagestyle{empty}
\begin{multicols*}{3}
\section{Boolean logic}

\section{Natural deduction}

\section{Structural induction}
Used to prove that some proposition P(x) holds for$\forall$ll x $\in$ recursively defined structure (e.g. lists, trees).

`\verb|()|' in Haskell changes the precedence (calling order) of functions. Nothing more.
\subsection*{Induction hypothesis}
\begin{itemize}
\item given as the known premise of a proof
\item ties recursive know in a proof
\item \textbf{must} be used
\end{itemize}
When proving, use only the below:
\begin{itemize}
\item the function definitions
\item the induction hypothesis
\item basic arithmetic
\end{itemize}
Sometimes prove from LHS to RHS; sometimes, from RHS to LHS; still sometimes, meet in the middle!
\subsection*{List induction rule}
\begin{displaymath}
\frac{P([])\qquad \forall x.\; \forall xs.\; P(xs) \rightarrow\; P(x:xs)}{\forall xs P(xs)}
\end{displaymath}
\begin{enumerate}
\item show that base case (empty list) $P([])$ holds
\item show that for any non-empty list (\verb|(x:xs)|) $P(x:xs)$ holds
\end{enumerate}
Step 2 \textbf{needs to use} induction hypothesis.

\subsection*{Choose proper formulation}
If a proof handles two or more lists, treat the one that remains unchanged in the definition(s) as \textbf{constant}:
\begin{lstlisting}
[] ++ ys = ys                       -- ( APP1 )
( x : xs ) ++ ys = x : ( xs ++ ys ) -- ( APP2 )
\end{lstlisting}
Then, choose induction on \texttt{xs} and treat \texttt{ys} as constant.
\subsection*{Len and map}
\begin{lstlisting}
length [] = 0                     -- ( LEN1 )
length ( x : xs ) = 1 + length xs -- ( LEN2 )

map f [] = []                     -- ( MAP1 )
map f ( x : xs ) = f x : map f xs -- ( MAP2 )
\end{lstlisting}

\subsection*{Tree induction rule}
\begin{displaymath}
\frac{P(Nul)\qquad \forall l.\; \forall x.\; \forall r.\; P(l) \land P(r) \rightarrow\; P(Node\,l\,x\,r:)}{\forall t.\; P(t)}
\end{displaymath}
\begin{enumerate}
\item show that base case (\verb|Node Nul|) $P(Nul)$ holds
\item show that $P(Node\;l\,x\,r)$ (\verb|Node lxr|) holds whenever both $P(l)$ and $P(r)$ are true
\end{enumerate}
\subsection*{Termination}

\section{Hoare logic}
%\input{lecs/lec5}
\end{multicols*}
\end{document}
